[EXTREMELY BROKEN] can we port the simple firewall
to support ip addresses of arbitrary lengths?

thy/Primitive_Matchers/Simple_Packet.thy
@@ -2,18 +2,25 @@ theory Simple_Packet
 imports "../Bitmagic/IPv4Addr" Protocol Conntrack_State
 begin
 
+
+(*TODO: how can I contain the typedef_overloaded?*)
+declare[[typedef_overloaded]]
+
 section{*Simple Packet*}
   text{*Packet constants are prefixed with @{text p}*}
-  record simple_packet = p_iiface :: string
+
+  text{*@{typ "'i::len word"} is an IP address of variable length. 32bit for IPv4, 128bit for IPv6*}
+
+  record 'i simple_packet = p_iiface :: string
                          p_oiface :: string
-                         p_src :: ipv4addr
-                         p_dst :: ipv4addr
+                         p_src :: "'i::len word"
+                         p_dst :: "'i::len word"
                          p_proto :: primitive_protocol
                          p_sport :: "16 word"
                          p_dport :: "16 word"
                          p_tcp_flags :: "tcp_flag set"
                          p_tag_ctstate :: ctstate
-print_theorems
+
 
   value "\<lparr>p_iiface = ''eth1'', p_oiface = '''', p_src = 0, p_dst = 0, p_proto = TCP, p_sport = 0, p_dport = 0, p_tcp_flags = {TCP_SYN}, p_tag_ctstate = CT_New\<rparr>"
 end
